Switch to use the new F* FFI interface
Switch to use the new F* FFI interface

libs/ml/FFICallbacks.ml
@@ -4,11 +4,11 @@ external ocaml_recv_tcp: callbacks -> string -> int = "ocaml_recv_tcp"
 
 (*module FFICallbacks = struct *)
   let recv sock maxlen =
-      let str = String.create maxlen in
+      let str = Bytes.create maxlen in
       let recvlen = ocaml_recv_tcp sock str in
       if recvlen < 0 then 
-        Platform.Error.Error("receive callback fail")
+        (0, Platform.Bytes.empty_bytes)
       else
         let str = String.sub str 0 recvlen in
-        Platform.Error.Correct(Platform.Bytes.abytes str)
+        (1, Platform.Bytes.abytes str)
 (* end *)
