libs/ml/FFICallbacks.mli
@@ -2,4 +2,4 @@ type callbacks = int
 val ocaml_send_tcp: callbacks -> string -> int
 val ocaml_recv_tcp: callbacks -> string -> int
 
-val recv: callbacks -> int -> (string, Platform.Bytes.bytes) Platform.Error.optResult 
+val recv: callbacks -> int -> (int * Platform.Bytes.bytes)
