src/tls/mitlsffi.h
@@ -18,7 +18,7 @@ extern int   FFI_mitls_configure(/* out */ mitls_state **state, const char *tls_
 // Close a miTLS session - either after configure or connect
 extern void FFI_mitls_close(/* in */ mitls_state *state);
 
-// Callbacks from miTLS to the host application, to send and receive TCP, invoked within FFI_mitls_connect() only
+// Callbacks from miTLS to the host application, to send and receive TCP
 struct _FFI_mitls_callbacks;
 typedef int (*pfn_FFI_send)(struct _FFI_mitls_callbacks *callbacks, const void *buffer, size_t buffer_size);
 typedef int (*pfn_FFI_recv)(struct _FFI_mitls_callbacks *callbacks, void *buffer, size_t buffer_size);
@@ -30,15 +30,15 @@ struct _FFI_mitls_callbacks {
 // Connect to a TLS server
 extern int   FFI_mitls_connect(struct _FFI_mitls_callbacks *callbacks, /* in */ mitls_state *state, /* out */ char **outmsg, /* out */ char **errmsg);
 
-// Prepare a plaintext packet for send over a TLS session
-extern void *FFI_mitls_prepare_send(/* in */ mitls_state *state, const void* buffer, size_t buffer_size, /* out */ size_t *packet_size, 
-                                    /* out */ char **outmsg, /* out */ char **errmsg); // Returns NULL for failure, or a TCP packet to be sent then freed with FFI_mitls_free_packet()
+// Send a message
+extern int FFI_mitls_send(/* in */ mitls_state *state, const void* buffer, size_t buffer_size,
+                            /* out */ char **outmsg, /* out */ char **errmsg); // Returns NULL for failure, or a TCP packet to be sent then freed with FFI_mitls_free_packet()
                                     
-// Decrypt a packet received over a TLS session
-extern void *FFI_mitls_handle_receive(/* in */ mitls_state *state, char* header, size_t header_size, char *record, size_t record_size, /* out */ size_t *packet_size, 
-                                      /* out */ char **outmsg, /* out */ char **errmsg);     // Returns NULL for failure, a plaintext packet to be freed with FFI_mitls_free_packet()
+// Receive a message
+extern void *FFI_mitls_receive(/* in */ mitls_state *state, /* out */ size_t *packet_size, 
+                               /* out */ char **outmsg, /* out */ char **errmsg);     // Returns NULL for failure, a plaintext packet to be freed with FFI_mitls_free_packet()
 
-// Free a packet returned from FFI_mitls_prepare_send() or FFI_mitls_handle_receive();
+// Free a packet returned FFI_mitls_receive();
 extern void FFI_mitls_free_packet(void* packet);
 
 // Free an outmsg or errmsg
