src/tls/FFI.fst
@@ -86,3 +86,4 @@ let write c msg : int =
 // the full shutdown (but many servers don't acknowledge).
 
 let close c = writeCloseNotify c
+
